added coercion for bool2prop, so the Coq translator no longer needs to insert it; added notations for Boolean-typed quantifiers such as "forallB"; started defining a semantics of specs using partial algebras
git-svn-id: svn+ssh://svn.kestrel.edu/Specware/branches/coq-branch@8632 7b97033b-253e-4a5c-9b07-e25f9089a9fd

Provers/ToCoq/MetaSlang.v
@@ -3,6 +3,7 @@
 
 Require Import String.
 Require Import Coq.Logic.Epsilon.
+Require Import Coq.Lists.List.
 
 
 (***
@@ -28,8 +29,16 @@ Fixpoint multi_arrow (types : list Type) (B : Type) : Type :=
 
 Axiom em_inf : forall (P : Prop), {P} + {~ P}.
 
-Definition bool2prop (b : bool) : Prop :=
-  b = true.
+Definition bool2prop (b : bool) : Prop := b = true.
+Coercion bool2prop : bool >-> Sortclass.
+
+Definition test1 : Prop := orb false true.
+(* Print test1. *)
+Lemma test1_pf : test1.
+  unfold test1.
+  reflexivity.
+Qed.
+
 
 Definition prop2bool (P : Prop) : bool :=
   match em_inf P with
@@ -37,41 +46,76 @@ Definition prop2bool (P : Prop) : bool :=
     | right _ => false
   end.
 
+(* unfortunately we can't do this... *)
+(* Coercion prop2bool : Prop >-> bool. *)
+
+(* We can do this, but it hardly seems worth it... *)
+(*
+Class MyProp : Type := myprop : Prop.
+Definition myProp2bool : MyProp -> bool := prop2bool.
+Coercion myProp2bool : MyProp >-> bool.
+Definition test2 : bool := (forall (X:Type) (x:X), x=x) : MyProp.
+*)
+
 Lemma prop2bool_true (P : Prop) (p : P) : prop2bool P = true.
   unfold prop2bool.
   case (em_inf P).
   intros; reflexivity.
-  intro notP; elimtype False; auto.
+  intro notP; elimtype False. apply notP; assumption.
 Qed.
 
 Lemma prop2bool_false (P : Prop) (notP : ~P) : prop2bool P = false.
   unfold prop2bool.
   case (em_inf P).
-  intro p; elimtype False; auto.
+  intro p; elimtype False. apply notP; assumption.
   intros; reflexivity.
 Qed.
 
+
+(***
+ *** deciding equality
+ ***)
+
 (* em_inf means that equality is decidable *)
-Definition dec_eq_pf (A : Set) (a b : A) : { a = b } + { ~ (a = b) } :=
+Definition dec_eq_pf {A : Set} (a b : A) : { a = b } + { ~ (a = b) } :=
   em_inf (a = b).
 
-Definition dec_eq_b (A : Set) (a b : A) : bool :=
+Definition dec_eq_b {A : Set} (a b : A) : bool :=
   prop2bool (a = b).
 
-Arguments dec_eq_b [A] _ _.
+Infix "==" := dec_eq_b (at level 70, no associativity).
 
 
 (***
  *** Coq versions of some basic Specware constructs
  ***)
 
-Definition the (A : Type) (p : { f : A -> bool | exists! x, f x = true })
+Definition the {A : Type} (p : { f : A -> bool | exists! x, f x })
 : { x : A | proj1_sig p x = true } :=
   constructive_definite_description
     (fun x => (proj1_sig p) x = true)
     (proj2_sig p).
 
-Arguments the [A] _.
+Definition forallb {A : Type} (f : A -> bool) : bool :=
+  prop2bool (forall x, f x).
+
+Notation "'forallB' x .. y , p" :=
+  (forallb (fun x => .. (forallb (fun y => p)) ..))
+    (at level 200, x binder, right associativity).
+
+Definition existsb {A : Type} (f : A -> bool) : bool :=
+  prop2bool (exists x, f x).
+
+Notation "'existsB' x .. y , p" :=
+  (existsb (fun x => .. (existsb (fun y => p)) ..))
+    (at level 200, x binder, right associativity).
+
+Definition existsb1 {A : Type} (f : A -> bool) : bool :=
+  prop2bool (exists! x, f x).
+
+Notation "'existsB' ! x .. y , p" :=
+  (existsb1 (fun x => .. (existsb1 (fun y => p)) ..))
+    (at level 200, x binder, right associativity).
 
 
 (***
@@ -104,6 +148,142 @@ Definition dec_neq_b_pair (p : bool * bool) :=
 (***
  *** The Spec type
  ***)
+
+(* a signature associates strings with types *)
+Definition Signature :=
+  list (string * Type).
+
+Inductive InSig : Signature -> string -> Type -> Prop :=
+| InSig_Base sig str T : InSig (cons (str, T) sig) str T
+| InSig_Cons sig str T str' T' :
+    InSig sig str T -> ~(str = str') -> InSig (cons (str', T') sig) str T.
+
+Definition SigString (sig : Signature) : Set :=
+  { str:string | exists T , InSig sig str T }.
+
+Program Fixpoint sig_lookup (sig : Signature) {struct sig}
+: SigString sig -> Type :=
+  match sig return { str:string | exists T , InSig sig str T } -> Type with
+    | (str', T) :: sig' =>
+      fun str =>
+        if string_dec str str' then T else sig_lookup sig' str
+    | nil => fun str_pair => string
+  end.
+Obligation 1.
+inversion H1.
+elimtype False; apply H; symmetry; assumption.
+exists H0; assumption.
+Defined.
+
+Lemma sig_lookup_insig_h :
+  forall (sig : Signature) (str : string) T
+         (insig : InSig sig str T)
+         (ex_T' : exists T' , InSig sig str T'),
+    sig_lookup sig (exist _ str ex_T') = T.
+  intros sig str T insig; induction insig; intro ex_T'.
+  unfold sig_lookup.
+  destruct
+    (string_dec
+       (proj1_sig
+          (exist
+             (fun str0 : string =>
+              exists T0 : Type, InSig ((str, T) :: sig) str0 T0) str ex_T'))).
+  reflexivity.
+  elimtype False; apply n; reflexivity.
+  unfold sig_lookup.
+  destruct
+    (string_dec
+       (proj1_sig
+          (exist
+             (fun str0 : string =>
+              exists T0 : Type, InSig ((str', T') :: sig) str0 T0) str ex_T'))).
+  elimtype False; apply H; assumption.
+  apply IHinsig.
+Qed.
+
+Lemma sig_lookup_insig :
+  forall (sig : Signature) (str : SigString sig) T,
+    InSig sig (proj1_sig str) T -> sig_lookup sig str = T.
+  intros sig str; destruct str as [ str insig' ].
+  intros T insig.
+  apply sig_lookup_insig_h.
+  assumption.
+Qed.
+
+(* subset relation on signatures *)
+Definition SigSubset (sig1 sig2 : Signature) : Prop :=
+  forall str T, InSig sig1 str T -> InSig sig2 str T.
+
+(* an algebra gives an element of each type in a sig *)
+Definition Algebra (sig : Signature) :=
+  forall (str : SigString sig), sig_lookup sig str.
+
+(* a partial algebra is one where only some elements are defined *)
+Definition PartialAlgebra (sig : Signature) :=
+  forall (str : SigString sig), option (sig_lookup sig str).
+
+(* an otion type refines to another one iff either the first is None
+   or both are equal *)
+Inductive OptRefinesTo {A : Type} : option A -> option A -> Prop :=
+| OptRefinesTo_None opt2 : OptRefinesTo None opt2
+| OptRefinesTo_Some a1 a2 : a1 = a2 -> OptRefinesTo (Some a1) (Some a2).
+
+(* a partial algebra refines to another iff the elements refine pointwise *)
+Definition PAlgRefinesTo {sig : Signature} (pa1 pa2 : PartialAlgebra sig) : Prop :=
+  forall (str : SigString sig), OptRefinesTo (pa1 str) (pa2 str).
+
+(* extension of partial alg refinement to fully-defined algebras *)
+Definition PAlgRefinesToAlg {sig : Signature}
+           (pa : PartialAlgebra sig) (a : Algebra sig) : Prop :=
+  forall (str : SigString sig), OptRefinesTo (pa str) (Some (a str)).
+
+(* a signature where all elements have type Set *)
+Definition SetSignature := list string.
+
+Definition SetSig2Sig : SetSignature -> Signature :=
+  map (fun str => (str, Set)).
+Coercion SetSig2Sig : SetSignature >-> Signature.
+
+(* FIXME: use sig_lookup_insig *)
+(*
+Lemma set_sig_lookup_is_set
+: forall (sig : SetSignature) str, sig_lookup sig str = Set.
+  intro sig; induction sig; intro str;
+  destruct str as [ str ex_insig ]; destruct ex_insig as [ T insig ].
+  inversion insig.
+  case_eq (string_dec str a).
+  intros e_str e_string_dec.
+  unfold sig_lookup; unfold SetSig2Sig; unfold map. rewrite e_string_dec.
+
+  unfold sig_lookup; unfold SetSig2Sig; unfold map; fold sig_lookup.
+  case_eq (string_dec (proj1_sig str) a).
+  intros e_str e_string_dec. rewrite e_str.
+rewrite e_string_dec.
+
+  destruct str as [ str ex_insig ].
+  destruct (dec_str )
+*)
+
+Definition DepSignature (sig : Signature)
+  := list (string * (Algebra sig -> Type)).
+
+Definition DepSigAsSig {sig : Signature}
+: DepSignature sig -> Signature :=
+  map (fun p => (fst p, forall alg, snd p alg)).
+
+Coercion DepSigAsSig : DepSignature >-> Signature.
+
+Definition Dep
+
+(* finally, the definition of a Spec! *)
+Record Spec :=
+  {
+    spec_types_sig : SetSignature;
+    spec_types : PartialAlgebra spec_types_sig;
+    spec_ops_sig : DependentSig spec_types_sig;
+    spec_ops : PartialAlgebra spec_ops_sig
+  }.
+
 
 (*
 Record Spec :=
